autoclrs/ch12-bst/c/BstDeleteKey.fst
@@ -1,4 +1,4 @@
-module BstMinMax
+module BstDeleteKey
 open Pulse
 open Pulse.Lib.C
 #lang-pulse
@@ -10,10 +10,11 @@ open CLRS.Ch12.BST.C.BridgeLemmas
 
 #restart-solver
 
-fn rec func_bst_minimum
+fn rec func_bst_search
     (var_keys: (array Int32.t))
     (var_valid: (array Int32.t))
     (var_cap: SizeT.t)
+    (var_key: Int32.t)
     (var_i: SizeT.t)
   requires
     exists* (val_keys_0: (Seq.seq (option Int32.t))) (val_keys_1: (nat->prop)).
@@ -26,13 +27,8 @@ fn rec func_bst_minimum
       (((reveal (length_of var_keys)) = (SizeT.v var_cap)) &&
         ((reveal (length_of var_valid)) = (SizeT.v var_cap))))
   requires (with_pure ((0 < (SizeT.v var_cap)) && ((SizeT.v var_cap) < 32768)))
-  requires
-    (with_pure
-      ((var_i `SizeT.lt` var_cap) &&
-        (not ((id #int (Int32.v ((array_read var_valid var_i)))) = 0))))
-  requires
-    (with_pure (c_valid_bst (array_value_of var_keys) (array_value_of var_valid) (SizeT.v var_cap)))
-  returns return_1 : Int32.t
+  requires (with_pure (var_i `SizeT.lte` var_cap))
+  returns return_1 : SizeT.t
   ensures
     exists* (val_keys_0: (Seq.seq (option Int32.t))) (val_keys_1: (nat->prop)).
     ((array_pts_to var_keys 1.0R val_keys_0 val_keys_1))
@@ -41,6 +37,12 @@ fn rec func_bst_minimum
     ((array_pts_to var_valid 1.0R val_valid_0 val_valid_1))
   ensures (with_pure ((reveal (length_of var_keys)) = (old (reveal (length_of var_keys)))))
   ensures (with_pure ((reveal (length_of var_valid)) = (old (reveal (length_of var_valid)))))
+  ensures (with_pure (return_1 `SizeT.lte` var_cap))
+  ensures
+    (with_pure
+      ((return_1 `SizeT.lt` var_cap) ==>
+        ((((array_read var_keys return_1)) = var_key) &&
+          (not ((id #int (Int32.v ((array_read var_valid return_1)))) = 0)))))
   ensures
     (with_pure
       (forall
@@ -53,32 +55,16 @@ fn rec func_bst_minimum
         (var_j: SizeT.t).
         ((var_j `SizeT.lt` var_cap) ==>
           (((array_read var_valid var_j)) = (old ((array_read var_valid var_j)))))))
-  ensures (with_pure (return_1 `Int32.lte` ((array_read var_keys var_i))))
   decreases (var_cap `SizeT.sub` var_i)
-{
-  let mut var_keys = var_keys;
-  let mut var_valid = var_valid;
-  let mut var_cap = var_cap;
-  let mut var_i = var_i;
-  let mut var_left : SizeT.t;
-  var_left := ((2sz `SizeT.mul` (!var_i)) `SizeT.add` 1sz);
-  if (((!var_cap) `SizeT.lte` (!var_left))) {
-    return ((array_read (!var_keys) (!var_i)));
-  } else {};
-  if ((((array_read (!var_valid) (!var_left))) = (Int32.int_to_t 0))) {
-    return ((array_read (!var_keys) (!var_i)));
-  } else {};
-  c_valid_bst_local_left (array_value_of (!var_keys)) (array_value_of (!var_valid)) (SizeT.v (!var_cap)) (SizeT.v (!var_i));
-  return (func_bst_minimum (!var_keys) (!var_valid) (!var_cap) (!var_left));
-}
+{ assume pure False; unreachable () }
 
 #restart-solver
 
-fn rec func_bst_maximum
+fn func_bst_delete
     (var_keys: (array Int32.t))
     (var_valid: (array Int32.t))
     (var_cap: SizeT.t)
-    (var_i: SizeT.t)
+    (var_del_idx: SizeT.t)
   requires
     exists* (val_keys_0: (Seq.seq (option Int32.t))) (val_keys_1: (nat->prop)).
     ((array_pts_to var_keys 1.0R val_keys_0 val_keys_1))
@@ -92,10 +78,8 @@ fn rec func_bst_maximum
   requires (with_pure ((0 < (SizeT.v var_cap)) && ((SizeT.v var_cap) < 32768)))
   requires
     (with_pure
-      ((var_i `SizeT.lt` var_cap) &&
-        (not ((id #int (Int32.v ((array_read var_valid var_i)))) = 0))))
-  requires
-    (with_pure (c_valid_bst (array_value_of var_keys) (array_value_of var_valid) (SizeT.v var_cap)))
+      ((var_del_idx `SizeT.lt` var_cap) &&
+        (not ((id #int (Int32.v ((array_read var_valid var_del_idx)))) = 0))))
   returns return_1 : Int32.t
   ensures
     exists* (val_keys_0: (Seq.seq (option Int32.t))) (val_keys_1: (nat->prop)).
@@ -107,31 +91,58 @@ fn rec func_bst_maximum
   ensures (with_pure ((reveal (length_of var_valid)) = (old (reveal (length_of var_valid)))))
   ensures
     (with_pure
-      (forall
-        (var_j: SizeT.t).
-        ((var_j `SizeT.lt` var_cap) ==>
-          (((array_read var_keys var_j)) = (old ((array_read var_keys var_j)))))))
+      (((id #int (Int32.v return_1)) = 0) ==>
+        (forall
+          (var_j: SizeT.t).
+          ((var_j `SizeT.lt` var_cap) ==>
+            (((array_read var_keys var_j)) = (old ((array_read var_keys var_j))))))))
   ensures
     (with_pure
-      (forall
-        (var_j: SizeT.t).
-        ((var_j `SizeT.lt` var_cap) ==>
-          (((array_read var_valid var_j)) = (old ((array_read var_valid var_j)))))))
-  ensures (with_pure (((array_read var_keys var_i)) `Int32.lte` return_1))
-  decreases (var_cap `SizeT.sub` var_i)
+      (((id #int (Int32.v return_1)) = 0) ==>
+        (forall
+          (var_j: SizeT.t).
+          ((var_j `SizeT.lt` var_cap) ==>
+            (((array_read var_valid var_j)) = (old ((array_read var_valid var_j))))))))
+{ assume pure False; unreachable () }
+
+#restart-solver
+
+fn func_bst_delete_key
+    (var_keys: (array Int32.t))
+    (var_valid: (array Int32.t))
+    (var_cap: SizeT.t)
+    (var_key: Int32.t)
+  requires
+    exists* (val_keys_0: (Seq.seq (option Int32.t))) (val_keys_1: (nat->prop)).
+    ((array_pts_to var_keys 1.0R val_keys_0 val_keys_1))
+  requires
+    exists* (val_valid_0: (Seq.seq (option Int32.t))) (val_valid_1: (nat->prop)).
+    ((array_pts_to var_valid 1.0R val_valid_0 val_valid_1))
+  requires
+    (with_pure
+      (((reveal (length_of var_keys)) = (SizeT.v var_cap)) &&
+        ((reveal (length_of var_valid)) = (SizeT.v var_cap))))
+  requires (with_pure ((0 < (SizeT.v var_cap)) && ((SizeT.v var_cap) < 32768)))
+  requires
+    (with_pure (c_valid_bst (array_value_of var_keys) (array_value_of var_valid) (SizeT.v var_cap)))
+  returns return_1 : Int32.t
+  ensures
+    exists* (val_keys_0: (Seq.seq (option Int32.t))) (val_keys_1: (nat->prop)).
+    ((array_pts_to var_keys 1.0R val_keys_0 val_keys_1))
+  ensures
+    exists* (val_valid_0: (Seq.seq (option Int32.t))) (val_valid_1: (nat->prop)).
+    ((array_pts_to var_valid 1.0R val_valid_0 val_valid_1))
+  ensures (with_pure ((reveal (length_of var_keys)) = (old (reveal (length_of var_keys)))))
+  ensures (with_pure ((reveal (length_of var_valid)) = (old (reveal (length_of var_valid)))))
 {
   let mut var_keys = var_keys;
   let mut var_valid = var_valid;
   let mut var_cap = var_cap;
-  let mut var_i = var_i;
-  let mut var_right : SizeT.t;
-  var_right := ((2sz `SizeT.mul` (!var_i)) `SizeT.add` 2sz);
-  if (((!var_cap) `SizeT.lte` (!var_right))) {
-    return ((array_read (!var_keys) (!var_i)));
+  let mut var_key = var_key;
+  let mut var_idx : SizeT.t;
+  var_idx := (func_bst_search (!var_keys) (!var_valid) (!var_cap) (!var_key) 0sz);
+  if (((!var_cap) `SizeT.lte` (!var_idx))) {
+    return (Int32.int_to_t 0);
   } else {};
-  if ((((array_read (!var_valid) (!var_right))) = (Int32.int_to_t 0))) {
-    return ((array_read (!var_keys) (!var_i)));
-  } else {};
-  c_valid_bst_local_right (array_value_of (!var_keys)) (array_value_of (!var_valid)) (SizeT.v (!var_cap)) (SizeT.v (!var_i));
-  return (func_bst_maximum (!var_keys) (!var_valid) (!var_cap) (!var_right));
+  return (func_bst_delete (!var_keys) (!var_valid) (!var_cap) (!var_idx));
 }
